src/Common.v
@@ -165,17 +165,17 @@ Ltac inversion_one_head T := inversion_one_match ltac:(destruct_head_matcher T).
 Ltac inversion_head' T := inversion_all_matches' ltac:(destruct_head_matcher T).
 
 
-Ltac destruct_head_hnf_matcher T HT :=
+Ltac head_hnf_matcher T HT :=
   match head_hnf HT with
     | T => idtac
   end.
-Ltac destruct_head_hnf T := destruct_all_matches ltac:(destruct_head_hnf_matcher T).
-Ltac destruct_one_head_hnf T := destruct_one_match ltac:(destruct_head_hnf_matcher T).
-Ltac destruct_head_hnf' T := destruct_all_matches' ltac:(destruct_head_hnf_matcher T).
+Ltac destruct_head_hnf T := destruct_all_matches ltac:(head_hnf_matcher T).
+Ltac destruct_one_head_hnf T := destruct_one_match ltac:(head_hnf_matcher T).
+Ltac destruct_head_hnf' T := destruct_all_matches' ltac:(head_hnf_matcher T).
 
-Ltac inversion_head_hnf T := inversion_all_matches ltac:(destruct_head_hnf_matcher T).
-Ltac inversion_one_head_hnf T := inversion_one_match ltac:(destruct_head_hnf_matcher T).
-Ltac inversion_head_hnf' T := inversion_all_matches' ltac:(destruct_head_hnf_matcher T).
+Ltac inversion_head_hnf T := inversion_all_matches ltac:(head_hnf_matcher T).
+Ltac inversion_one_head_hnf T := inversion_one_match ltac:(head_hnf_matcher T).
+Ltac inversion_head_hnf' T := inversion_all_matches' ltac:(head_hnf_matcher T).
 
 Ltac destruct_sig_matcher HT :=
   match eval hnf in HT with
